
\documentclass{article}
\usepackage{style}

\begin{document}

\begin{question}

\[ 1+3+5+\cdots+(2n-1) = n^2 \]

\begin{align*}
\stext{Prove for \(n=4\)}
1+3+5+(2(4)-1) &= 1+3+5+7 \\[8pt]
&= 16 \\[8pt]
&= 4^{2} \\[8pt]
\stext{assume \(n=k\) holds true}
1+3+5+\cdots+(2k-1)=k^{2}\\[8pt]
\stext{Prove for \(n=k+1\)}
1+3+5+(2k-1)+(2(k+1)-1) &= 1+3+5+\cdots+(2k-1)+(2(k+1)-1) \\[8pt]
&= k^{2}+(2(k+1)-1) \\[8pt]
&= k^{2}+(2k+2-1) \\[8pt]
&= k^{2}+2k+1 \\[8pt]
&= (k+1)^{2} \\[8pt]
\stext{Thus, the statement holds true for \(n=k+1\) if it holds true for \(n=k\).}\\[8pt]
\end{align*}

\end{question}

\begin{question}

\[5^{n} \text{always ends in a \(5\)}\]

\begin{align*}
\stext{Prove for \(n=1\)}
5^{1} &= 5 \\[8pt]
\stext{assume \(n=k\) holds true}
5^{k} &= \text{ends in a \(5\)}\\[8pt]
\stext{Prove for \(n=k+1\)}
5^{k+1} &= 5^{k} \cdots 5 \\[8pt]
&= \text{ends in a \(5\)} \cdot 5 \\[8pt]
&= \text{ends in a \(5\)} \\[8pt]
\stext{Thus, the statement holds true for \(n=k+1\)}
\end{align*}

\end{question}

\begin{question}

\[7^{n} -1 = 6m\]

\begin{align*}
\stext{Prove for \(n=1\)}
7^{1} - 1 &= 6 \\[8pt]
\stext{Assume \(n=k\) holds true}
7^{k} - 1 &= 6m \\[8pt]
\stext{Prove for \(n=k+1\)}
7^{k+1} - 1 &= 7 \cdot 7^{k} -1\\[8pt]
&= 7(6m + 1) - 1 \\[8pt]
&= 42m + 7 - 1 \\[8pt]
&= 42m + 6 \\[8pt]
&= 6(7m + 1) \\[8pt]
&= 6m' \\[8pt]
\stext{where \(m' = 7m + 1\)}\\[8pt]
\stext{Thus, the statement holds true for \(n=k+1\)}
\end{align*}

\end{question}

\begin{question}

\[ 2^{n} \geq n+1 \]

\begin{align*}
\stext{Prove for \(n=1\)}
2^{1} &\geq 1+1 \\[8pt]
&= 2 \\[8pt]    
\stext{assume \(n=k\) holds true}
2^{k} &\geq k+1 \\[8pt]
\stext{Prove for \(n=k+1\)}
2^{k+1} &\geq k+1 +1\\[8pt]
&\geq k+2\\[8pt]
k+1 &\geq \frac{k+2}{2}\\[8pt]
&\geq \frac{k}{2} + 1\\[8pt]
\stext{Thus, the statement holds true for \(n=k+1\) if it holds true for \(n=k\).}\\[8pt]
\end{align*}

\end{question}

\begin{question}

\[ 1^3+2^3+3^3+\cdots+n^3 = \left(\frac{n(n+1)}{2}\right)^2 \]

\begin{align*}
\stext{Prove for \(n=1\)}
1^3 &= \left(\frac{1(1+1)}{2}\right)^2 \\[8pt]
&= \left(\frac{1 \cdot 2}{2}\right)^2 \\[8pt]
&= 1^2 \\[8pt]
&= 1 \\[8pt]
\stext{assume \(n=k\) holds true}
1^3+2^3+\cdots+k^3 &= \left(\frac{k(k+1)}{2}\right)^2 \\[8pt]
\stext{Prove for \(n=k+1\)}
1^3+2^3+\cdots+k^3+(k+1)^3 &= \left(\frac{k(k+1)}{2}\right)^2 + (k+1)^3 \\[8pt]
&= \left(\frac{k(k+1)}{2}\right)^2 + (k+1)(k+1)(k+1) \\[8pt]
&= \left(\frac{k(k+1)}{2}\right)^2 + (k+1)^3 \\[8pt]
&= \left(\frac{k(k+1)}{2}\right)^2 + k^3 +3k^2 + 3k + 1 \\[8pt]
\end{align*}

\end{question}

\end{document}